Reworked definitions to better reuse them for defining eval

asign6.v
@@ -19,7 +19,7 @@ Open Scope LangContext_scope.
 
 Lemma Weakening {Γ1 e τ Γ2} (sub: Γ1 ⊆ Γ2) : Γ1 ⊢ e ∷ τ -> Γ2 ⊢ e ∷ τ.
   by rewrite sub.
-Qed.
+Defined.
 
 Ltac weakening := apply/Weakening/(SubContextConsRight (SubContextRefl _)).
 
@@ -30,29 +30,36 @@ Lemma OtherWeakening {s e} (sNotIn : s ∉f e) : forall {Γ τ} (typechecks1 : �
   - by apply/(EquivContextAlsoTypechecks (H _ _ type1 τ'))/EquivContextP => ? /=; program_equiv.
   - by apply/(EquivContextAlsoTypechecks type1)/EquivContextP => ? /=; program_equiv.
   - by apply/(EquivContextAlsoTypechecks type1)/EquivContextP => ? /=; program_equiv.
-Qed.
+Defined.
 
 Hint Resolve (@OtherWeakening).
 Hint Resolve (@Weakening).
 
-Lemma Substitution {e1 Γ1 τ1} (typechks1 : Γ1 ⊢ e1 ∷ τ1) : forall e2 e3 Γ2 τ2 s,
-  (s ∷ τ2 ∈ Γ1) -> Γ2 ⊢ e2 ∷ τ2 -> Γ1 ≡ Γ2 % s -> [e2 / s] e1 = e3 -> Γ2 ⊢ e3 ∷ τ1.
-  elim: typechks1; intros; match goal with | H : [ _ / _ ] _ = _ |- _ => inversion H end; subst.
+Hint Resolve InContextUnique.
+
+Lemma Substitution {e1 Γ1 τ1} (typechks1 : Γ1 ⊢ e1 ∷ τ1) : forall e2 e3 Γ2 τ2 s
+  (in1: s ∷ τ2 ∈ Γ1) (ty2: Γ2 ⊢ e2 ∷ τ2) (cong: Γ1 ≡ Γ2 % s) (sub: [e2 / s] e1 = e3), Γ2 ⊢ e3 ∷ τ1.
+  induction typechks1; intros; inversion sub; subst.
   1,4,5,7,8: done.
-  - by move/InContextP in H; move/InContextP in H0.
-  - by move/(InterpretCongMod H2 neq) in H.
-  - by have: s ∷ τ2 ∈ (ConsEnv x τarg (ConsEnv f (τarg → τret) Γ)) /\
-             (ConsEnv x τarg (ConsEnv f (τarg → τret) Γ2)) ⊢ e2 ∷ τ2 by done.
-Qed.
+  - by have: τ=τ2.
+  - by have: s ∷ τ ∈ Γ2 by rewrite -InterpretCongMod.
+  - by have: let G Γ := (ConsEnv x τarg (ConsEnv f (τarg → τret) Γ)) in s ∷ τ2 ∈ (G Γ) /\ (G Γ2) ⊢ e2 ∷ τ2.
+Defined.
 
 Lemma CannonicalForms {Γ e τ} :
   Γ ⊢ e ∷ τ -> forall (v: 𝕍 e),
   match τ with
-  | NatType => exists n, e = (NatExpr n)
-  | (AbsType τ1 τ2) => exists f x body, f<>x /\ (e = (AbsExpr f x τ1 τ2 body))
+  | NatType => {n | e = (NatExpr n)}
+  | (AbsType τ1 τ2) => {tup  | match tup with (f, x, body) => f<>x /\ (e = (AbsExpr f x τ1 τ2 body)) end}
   end.
-  by case.
-Qed.
+  move/TypechecksP.
+  functional inversion 1; try done.
+  intros vabs.
+  exists (f, x, body).
+  done.
+  Unshelve.
+  all: done.
+Defined.
 
 Ltac Cannonicalize := repeat (match goal with
                               | V: 𝕍 ?e, T: _ ⊢ ?e ∷ _ |- _ =>
@@ -61,59 +68,122 @@ Ltac Cannonicalize := repeat (match goal with
 
 Lemma TypedEvalContextInversion {Γ E τ0 τ} : Γ ⊢ E {τ0} ∷ τ -> exists x, x ∉ Γ /\ (ConsEnv x τ0 Γ) ⊢ E[x] ∷ τ.
   by induction 1; simpl; first by destruct (ContextFinite Γ).
-Qed.
+Defined.
 
-Lemma TypedBinopExprInversion {Γ f e1 e2 τ} : Γ ⊢ (BinExpr f e1 e2) ∷ τ -> exists τ1 τ2, Γ ⊢ e1 ∷ τ1 /\ Γ ⊢ e2 ∷ τ2.
-  by inversion 1.
-Qed.
+Lemma TypedBinopExprInversion {Γ f e1 e2 τ} : Γ ⊢ (BinExpr f e1 e2) ∷ τ -> {τ1 | Γ ⊢ e1 ∷ τ1} * {τ2 | Γ ⊢ e2 ∷ τ2}.
+  move/TypechecksP => typ.
+  by functional inversion typ; subst; repeat match goal with H : (typchk _ _) = _ |- _ => move/TypechecksP in H end.
+Defined.
 
 Lemma DecompositionOfTypes E : forall Γ e0 τ, Γ ⊢ E[e0] ∷ τ -> exists τ1, Γ ⊢ e0 ∷ τ1 /\ Γ ⊢ E {τ1} ∷ τ.
   induction E; intros; simpl in *; first done.
   all: inversion H.
   1,2: by move/IHE: type1 => [τx [? b]]; move:(TypedEvalContextInversion b).
   1,2: move/IHE: type2 => [τx [? b]]; move:(TypedEvalContextInversion b); Cannonicalize => //=.
-  by intros; elim_exists; case: H6 => ?; case.
-Qed.
+  intros; elim_exists.
+  inversion CannonicalForms0.
+  destruct x1.
+  destruct p.
+  case: H6 => ?; case.
+  done.
+Defined.
 
-Definition CanStep e := exists e', e ⥛ e'.
-Definition CanStepEβ e := exists E e0 e1, e=E[e0] /\ e0 ⥛β e1.
-Definition CanStepβ e := exists e', e ⥛β e'.
+Definition CanStep e := exists e0, e ⥛ e0.
+Definition CanStepβ e := exists e0, e ⥛β e0.
+Definition CanStepEβ e := exists E e0, e=E[e0] /\ CanStepβ e0.
 Definition NotStuck e := 𝕍 e \/ (CanStep e).
-Definition NotStuckEβ e := 𝕍 e \/ (CanStepEβ e).
 Definition NotStuckβ e := 𝕍 e \/ (CanStepβ e).
+Definition NotStuckEβ e := 𝕍 e \/ (CanStepEβ e).
 
 Hint Constructors EvaluationContext.
 
 Ltac CAS := apply/CASAlways/AlwaysSafeToSubInto.
 
-Lemma ProgressApp {Γ e1 e2 τ} : Γ ⊢ (BinExpr AppExpr e1 e2) ∷ τ -> (𝕍 e1) -> (𝕍 e2) -> exists e, (BinExpr AppExpr e1 e2) ⥛β e.
-  inversion 1.
-  move/(CannonicalForms type1) => [f [x [body [? ?]]]] v2.
-  have: exists b, [e2 / x] body = b by CAS.
+Lemma ProgressApp {Γ e1 e2 τ} : Γ ⊢ (BinExpr AppExpr e1 e2) ∷ τ -> (𝕍 e1) -> (𝕍 e2) -> {e0 | (BinExpr AppExpr e1 e2) ⥛β e0}.
+  move/TypechecksP => typ.
+  functional inversion typ; subst; repeat (match goal with | H : (typchk _ _) = _ |- _ => move/TypechecksP in H end).
+  move/(CannonicalForms H3) => [[[f x] body] [? ?]] v2.
+  have: {b | [e2 / x] body = b} by CAS.
   move => [x0 ?].
-  have: exists b, [(AbsExpr f x τ1 τ body) / f] x0 = b by CAS.
+  have: {b | [(AbsExpr f x τa1 τ body) / f] x0 = b} by CAS.
+  move => [x1 ?].
   done.
-Qed.
+Defined.
 
-Lemma ProgressBin : forall f {e1 e2 Γ τ} (typ: Γ ⊢ (BinExpr f e1 e2) ∷ τ) (v1 : 𝕍 e1) (v2 : 𝕍 e2), NotStuckβ (BinExpr f e1 e2).
-  case => e1 e2 Γ τ typ v1 v2.
-  - by inversion typ; Cannonicalize.
-  - right; exact/ProgressApp.
-Qed.
+Lemma ProgressBin : forall f {e1 e2 Γ τ} (typ: Γ ⊢ (BinExpr f e1 e2) ∷ τ) (v1 : 𝕍 e1) (v2 : 𝕍 e2), {e0 | (BinExpr f e1 e2) ⥛β e0}.
+  move => f e1 e2 Γ τ typ v1 v2.
+  move/TypechecksP in typ.
+  functional inversion typ; subst; repeat (match goal with | H : (typchk _ _) = _ |- _ => move/TypechecksP in H end).
+  - by move: (CannonicalForms H4 v1) (CannonicalForms H5 v2) => [n0 ->] [n1 ->].
+  - exact/ProgressApp.
+Defined.
 
-Lemma Progressβ : forall {e τ} (ety: NullEnv ⊢ e ∷ τ), NotStuckEβ e.
-  induction e => τ //=.
-  - inversion 1; inversion H1.
-  - move=>ty; move/TypedBinopExprInversion: (ty) => [τ1 [τ2 [/IHe1-[v1|p1] /IHe2 ns2]]].
-    + case: ns2 => [v2|p2].
-      * by move: (ProgressBin ty v1 v2) => [//= | [e s]]; right; exists Hole.
-      * by move: p2 => [E [e0 [e3 [-> s]]]]; right; exists (EvalContextBinR f v1 E).
-    + by move: p1 => [E [e0 [e3 [-> s]]]]; right; exists (EvalContextBinL f E e2).
-Qed.
+Record SteppableDecomposedExpr (e : 𝔼) : Set :=
+  mkDecomposed {
+      DContext : EvaluationContext ;
+      DExpr : 𝔼 ;
+      DIsDecomp : e = DContext[DExpr] ;
+      DSteps : {e0 | DExpr ⥛β e0}
+    }.
+
+Lemma ValDec : forall e, decidable (𝕍 e).
+  by case.
+Defined.
+
+Program Fixpoint EvalContextDecomp e (nv : ~ 𝕍 e) (τ: {τ | NullEnv ⊢ e ∷ τ}) {struct e} : SteppableDecomposedExpr e :=
+  match e with
+  | VarExpr _ => _
+  | NatExpr n => _
+  | AbsExpr _ _ _ _ _ => _
+  | BinExpr op l r =>
+    match (ValDec l) with
+    | left vl => 
+      match (ValDec r) with
+      | left vr => 
+        @mkDecomposed e Hole e _ _
+      | right nvr =>
+        let decomp := (EvalContextDecomp _ _) in
+        @mkDecomposed e (EvalContextBinR op vl (DContext decomp)) (DExpr decomp) _ _
+      end
+    | right nvl =>
+      let decomp := (@EvalContextDecomp l _ _) in
+      @mkDecomposed e (EvalContextBinL op (DContext decomp) r) (DExpr decomp) _ _
+    end
+  end.
+Next Obligation.
+  suff: forall s τ, NullEnv ⊢ (VarExpr s) ∷ τ -> False by move=> /(_ wildcard' τ).
+  move=> s τ0; inversion 1; inversion H3.
+Defined.
+Next Obligation.
+  case (nv (NatValue n)).
+Defined.
+Next Obligation.
+  case (nv (AbsValue _ _ _ _ _)).
+Defined.
+Next Obligation.
+  exact (ProgressBin H vl vr).
+Defined.
+Next Obligation.
+  simpl.
+  move/TypedBinopExprInversion in H.
+  inversion H.
+  inversion H1.
+  done.
+Defined.
+Next Obligation.
+  by simpl in *; move/TypedBinopExprInversion in H.
+Defined.
+
+Lemma Progressβ {e τ} (ety: NullEnv ⊢ e ∷ τ) : NotStuckEβ e.
+  induction e => //=.
+  - inversion ety; inversion H1.
+  - have: ~ (𝕍 (BinExpr f e1 e2)) by done.
+    by move=> nv; destruct (EvalContextDecomp nv ltac:(done)); move: DSteps0 => [e0 step].
+Defined.
 
 Lemma Progress {e} : forall {τ} (etyp: NullEnv ⊢ e ∷ τ), (NotStuck e).
-  by move=> τ /Progressβ; move=> [v | [E [e0 [e1 [-> bstep]]]]].
-Qed.
+    by move=> τ /Progressβ; move=> [v | [E [e0 [-> [e1 bstep]]]]].
+Defined.
 
 Hint Resolve Progress.
 
@@ -122,7 +192,7 @@ Lemma βPreservation {e e'} (estep : e ⥛β e') : forall τ (etyp : NullEnv ⊢
   subst; inversion type1; subst.
   (have: ((ConsEnv f (τ1 → τ0) NullEnv) ⊢ e ∷ τ1) by done) => ?.
   by apply/Substitution; first by apply/Substitution.
-Qed.
+Defined.
 
 Hint Resolve βPreservation.
 
@@ -130,12 +200,92 @@ Hint Resolve InterpretTypedEvalContext.
 
 Lemma Preservation {e e'} (estep : e ⥛ e') τ (etyp : NullEnv ⊢ e ∷ τ) : NullEnv ⊢ e' ∷ τ.
   by inversion estep; subst; move: (DecompositionOfTypes E e1 etyp).
-Qed.
+Defined.
 
 Hint Resolve Preservation.
 
 Lemma Safety {e τ} (etyp : NullEnv ⊢ e ∷ τ) {e'} (estep : e ⥛* e') : (NotStuck e').
   by induction estep.
-Qed.
+Defined.
+
+Lemma Preservation0 {e e0} (estep : e ⥛ e0) : {τ | NullEnv ⊢ e ∷ τ} -> {τ | NullEnv ⊢ e0 ∷ τ}.
+  inversion 1.
+  econstructor.
+  by apply/Preservation.
+Defined.
+
+CoInductive Stream (A: Type) : Type :=
+| SNil : Stream A
+| SCons (e : A) (tl: Stream A) : Stream A.
+
+CoFixpoint Evaluate (e : 𝔼) (τ : {τ | NullEnv ⊢ e ∷ τ}) : Stream 𝔼.
+  refine (match (ValDec e) with
+          | left v => SNil 𝔼
+          | right nv => let decomp := EvalContextDecomp nv τ in
+                       let: (exist _ e0 step) := (DSteps decomp) in
+                       let newe := (DContext decomp)[e0] in
+                       SCons newe (@Evaluate newe (Preservation0 (@ECSS (DContext decomp) (DExpr decomp) e0 step) _))
+          end).
+  by rewrite <- (DIsDecomp decomp).
+Defined.
+
+Fixpoint approx {A} (s : Stream A) (n : nat) : list A :=
+  match n with
+    | O => nil
+    | S n' =>
+      match s with
+        | SCons h t => h :: approx t n'
+        | SNil _ => nil
+      end
+  end.
+
+Definition Evaluate0 (e : 𝔼) : Stream 𝔼.
+  refine ((match (typchk NullEnv e) as st return ((typchk NullEnv e) = st -> _) with
+           | (Some τ) => (fun (eq: (typchk NullEnv e) = (Some τ)) => _)
+           | None => (fun (eq: (typchk NullEnv e) = None) => SNil 𝔼)
+           end) (eq_refl (typchk NullEnv e))).
+  by move/TypechecksP in eq; apply/Evaluate.
+Defined.
+Set Printing Implicit.
+Eval vm_compute in (approx (Evaluate0 (BinExpr AddExpr 5 5)) 3).
+match
+         (let
+          'exist _ e0 step :=
+           ProgressBin (iffRL (P:=NullEnv ⊢ (5 + 5) ∷ ℕ) TypechecksP (erefl (Some NatType))) (NatValue 5) (NatValue 5) in
+           SCons e0
+             (Evaluate
+                (exist [eta Typechecks NullEnv e0] NatType
+                   (InterpretTypedEvalContext (TypedHole NullEnv ℕ)
+                      (βPreservation step (iffRL (P:=NullEnv ⊢ (5 + 5) ∷ ℕ) TypechecksP (erefl (Some NatType))))))))
+       with
+       | SNil _ => nil
+       | SCons h t =>
+           h :: match t with
+                | SNil _ => nil
+                | SCons h0 t0 => h0 :: match t0 with
+                                       | SNil _ => nil
+                                       | SCons h1 _ => h1 :: nil
+                                       end
+                end
+       end
+Eval eta in (match
+                  (let 'exist _ e0 step :=
+                       ProgressBin (iffRL (P:=NullEnv ⊢ (5 + 5) ∷ ℕ) TypechecksP (erefl (Some NatType))) (NatValue 5) (NatValue 5) in
+                   SCons e0
+                         (Evaluate
+                            (Preservation0 (ECSS step)
+                                           (exist (fun x => Typechecks NullEnv Hole [(5 + 5)] x) NatType
+                                                  (iffRL (P:=NullEnv ⊢ (5 + 5) ∷ ℕ) TypechecksP (erefl (Some NatType)))))))
+          with
+          | SNil _ => nil
+          | SCons h t => h :: match t with
+                             | SNil _ => nil
+                             | SCons h0 _ => h0 :: nil
+                             end
+                end).
+
+
+
+
 
 
